fstar/new/TreeSyncTreeKEMBinder.fst
@@ -9,6 +9,8 @@ module TS = TreeSync
 module TK = TreeKEM
 open Lib.Result
 
+#set-options "--fuel 1 --ifuel 1"
+
 //TODO I guess this is somewhere in the standard library
 val pub_to_secret: pb:pub_bytes -> b:bytes{Seq.length b == Seq.length pb}
 let pub_to_secret pb =
@@ -59,8 +61,8 @@ let ps_node_package_content =
     (fun (|public_key, (|encrypted_path_secret, last_group_context|)|) -> ({npc_public_key = public_key; npc_encrypted_path_secret = encrypted_path_secret; npc_last_group_context = last_group_context;}))
     (fun x -> (|x.npc_public_key, (|x.npc_encrypted_path_secret, x.npc_last_group_context|)|))
 
-val treesync_to_treekem: #l:nat -> #n:tree_size l -> cs:ciphersuite -> TS.treesync l n -> result (TK.treekem cs l n)
-let rec treesync_to_treekem #l #n cs t =
+val treesync_to_treekem_aux: #l:nat -> #n:tree_size l -> cs:ciphersuite -> nat -> TS.treesync l n -> result (TK.treekem cs l n)
+let rec treesync_to_treekem_aux #l #n cs nb_left_leaves t =
   match t with
   | TLeaf (_, None) ->
     return (TLeaf None)
@@ -72,11 +74,11 @@ let rec treesync_to_treekem #l #n cs t =
     else
       fail "treesync_to_treekem: public key has wrong length"
   | TSkip _ t' ->
-    result <-- treesync_to_treekem cs t';
+    result <-- treesync_to_treekem_aux cs nb_left_leaves t';
     return (TSkip _ result)
   | TNode (_, onp) left right -> begin
-    tk_left <-- treesync_to_treekem cs left;
-    tk_right <-- treesync_to_treekem cs right;
+    tk_left <-- treesync_to_treekem_aux cs nb_left_leaves left;
+    tk_right <-- treesync_to_treekem_aux cs (nb_left_leaves + pow2 (l-1)) right;
     match onp with
     | None ->
       return (TNode None tk_left tk_right)
@@ -84,6 +86,12 @@ let rec treesync_to_treekem #l #n cs t =
       content <-- from_option "treesync_to_treekem: Couldn't parse node content"
         ((ps_to_pse ps_node_package_content).parse_exact (pub_to_secret np.TS.np_content));
       path_secret_ciphertext <-- mapM (encrypted_path_secret_nt_to_tk cs) (Seq.seq_to_list content.npc_encrypted_path_secret);
+      unmerged_leaves <-- mapM (fun (unmerged_leaf:nat) ->
+        if not (nb_left_leaves <= unmerged_leaf) then
+          fail "treesync_to_treekem: unmerged_leaf index too big"
+        else
+          return ((unmerged_leaf - nb_left_leaves) <: nat)
+      ) np.TS.np_unmerged_leafs;
       if not (Seq.length content.npc_public_key = hpke_public_key_length cs) then
         fail ""
       else (
@@ -91,13 +99,17 @@ let rec treesync_to_treekem #l #n cs t =
           TK.kp_public_key = content.npc_public_key;
           TK.kp_version = np.TS.np_version;
           TK.kp_last_group_context = content.npc_last_group_context;
-          TK.kp_unmerged_leafs = np.TS.np_unmerged_leafs;
+          TK.kp_unmerged_leafs = unmerged_leaves;
           TK.kp_path_secret_from = (np.TS.np_content_dir);
           TK.kp_path_secret_ciphertext = path_secret_ciphertext;
         } in
         return (TNode (Some kp) tk_left tk_right)
       )
   end
+
+val treesync_to_treekem: #l:nat -> #n:tree_size l -> cs:ciphersuite -> TS.treesync l n -> result (TK.treekem cs l n)
+let treesync_to_treekem #l #n cs t =
+  treesync_to_treekem_aux cs 0 t
 
 let encrypted_path_secret_tk_to_nt (#cs:ciphersuite) (x:TK.path_secret_ciphertext cs): result (hpke_ciphertext_nt) =
   if not (Seq.length x.TK.kem_output < pow2 16) then
@@ -111,8 +123,9 @@ let encrypted_path_secret_tk_to_nt (#cs:ciphersuite) (x:TK.path_secret_ciphertex
     })
 
 
-val treekem_to_treesync: #l:nat -> #n:tree_size l -> #i:leaf_index n -> #cs:ciphersuite -> TS.leaf_package_t -> TK.pathkem cs l n i -> result (TS.pathsync l n i)
-let rec treekem_to_treesync #l #cs old_leaf_package p =
+#push-options "--z3rlimit 50"
+val treekem_to_treesync_aux: #l:nat -> #n:tree_size l -> #i:leaf_index n -> #cs:ciphersuite -> nat -> TS.leaf_package_t -> TK.pathkem cs l n i -> result (TS.pathsync l n i)
+let rec treekem_to_treesync_aux #l #n #i #cs nb_left_leaves old_leaf_package p =
   match p with
   | PLeaf mi ->
     return (PLeaf (Some ({
@@ -125,10 +138,12 @@ let rec treekem_to_treesync #l #cs old_leaf_package p =
       TS.lp_signature = old_leaf_package.TS.lp_signature; //TODO the signature definitely has to change
     })))
   | PSkip _ p' ->
-    result <-- treekem_to_treesync old_leaf_package p';
+    result <-- treekem_to_treesync_aux nb_left_leaves old_leaf_package p';
     return (PSkip _ result)
   | PNode kp p_next ->
-    next <-- treekem_to_treesync old_leaf_package p_next;
+    let (|dir, _|) = child_index l i in
+    let new_left_leaves = (if dir = Left then nb_left_leaves else nb_left_leaves + pow2 (l-1)) in
+    next <-- treekem_to_treesync_aux new_left_leaves old_leaf_package p_next;
     ciphertexts <-- mapM encrypted_path_secret_tk_to_nt kp.TK.kp_path_secret_ciphertext;
     if not (byte_length ps_hpke_ciphertext ciphertexts < pow2 16) then
       fail "treekem_to_treesync: ciphertexts too long"
@@ -144,12 +159,17 @@ let rec treekem_to_treesync #l #cs old_leaf_package p =
       let np = ({
         TS.np_version = kp.TK.kp_version;
         TS.np_content_dir = kp.TK.kp_path_secret_from;
-        TS.np_unmerged_leafs = kp.TK.kp_unmerged_leafs;
+        TS.np_unmerged_leafs = List.Tot.map (fun (x:nat) -> (x + nb_left_leaves <: nat)) kp.TK.kp_unmerged_leafs;
         TS.np_parent_hash = bytes_empty; //The parent hash needs to be recomputed
         TS.np_content = secret_to_pub np_content;
       }) in
       return (PNode (Some np) next)
     end
+#pop-options
+
+val treekem_to_treesync: #l:nat -> #n:tree_size l -> #i:leaf_index n -> #cs:ciphersuite -> TS.leaf_package_t -> TK.pathkem cs l n i -> result (TS.pathsync l n i)
+let treekem_to_treesync #l #n #i #cs old_leaf_package p =
+  treekem_to_treesync_aux 0 old_leaf_package p
 
 (*** NetworkTreeSyncBinder ***)
 //TODO move this in an other file
@@ -212,6 +232,67 @@ let treesync_to_parent_node np =
       pnn_parent_hash = np.TS.np_parent_hash;
       pnn_unmerged_leaves = Seq.seq_of_list unmerged_leaves;
     })
+  )
+
+val key_package_to_treekem: cs:ciphersuite -> key_package_nt -> result (TK.member_info cs)
+let key_package_to_treekem cs kp =
+  if not (Seq.length kp.kpn_public_key = hpke_public_key_length cs) then
+    fail "key_package_to_treekem: public key has wrong length"
+  else
+    return ({
+      TK.mi_public_key = kp.kpn_public_key;
+      TK.mi_version = 0;
+    })
+
+val update_path_node_to_treekem: cs:ciphersuite -> bytes -> direction -> update_path_node_nt -> result (TK.key_package cs)
+let update_path_node_to_treekem cs group_context dir update_path_node =
+  if not (Seq.length update_path_node.upnn_public_key = hpke_public_key_length cs) then
+    fail "update_path_node_to_treekem: public key has wrong length"
+  else (
+    path_secret_ciphertext <-- mapM (fun hpke_ciphertext ->
+      if not (Seq.length hpke_ciphertext.hcn_kem_output = hpke_kem_output_length cs) then
+        fail "update_path_node_to_treekem: kem output has wrong length"
+      else
+        return ({
+          TK.kem_output = hpke_ciphertext.hcn_kem_output;
+          TK.ciphertext = hpke_ciphertext.hcn_ciphertext;
+        })
+    ) (Seq.seq_to_list update_path_node.upnn_encrypted_path_secret);
+    return ({
+      TK.kp_public_key = update_path_node.upnn_public_key;
+      TK.kp_version = 0;
+      TK.kp_last_group_context = group_context;
+      TK.kp_unmerged_leafs = [];
+      TK.kp_path_secret_from = dir;
+      TK.kp_path_secret_ciphertext = path_secret_ciphertext;
+    })
+  )
+
+val update_path_to_treekem: cs:ciphersuite -> l:nat -> n:tree_size l -> i:leaf_index n -> bytes -> update_path:update_path_nt -> result (TK.pathkem cs l n i)
+let rec update_path_to_treekem cs l n i group_context update_path =
+  if l = 0 then (
+    if not (Seq.length update_path.upn_nodes = 0) then
+      fail "update_path_to_treekem: update_path.nodes is too long"
+    else (
+      leaf_package <-- key_package_to_treekem cs update_path.upn_leaf_key_package;
+      return (PLeaf leaf_package)
+    )
+  ) else if (n <= pow2 (l-1)) then (
+    path_next <-- update_path_to_treekem cs (l-1) n i group_context update_path;
+    return (PSkip _ path_next)
+  ) else (
+    if not (Seq.length update_path.upn_nodes > 0) then
+      fail "update_path_to_treekem: update_path.nodes is too short"
+    else (
+      let update_path_length = (Seq.length update_path.upn_nodes) in
+      let head_update_path_nodes = Seq.index update_path.upn_nodes (update_path_length-1) in
+      let tail_update_path_nodes = Seq.slice update_path.upn_nodes 0 (update_path_length-1) in
+      let next_update_path = { update_path with upn_nodes = tail_update_path_nodes } in
+      let (|dir, next_i|) = child_index l i in
+      path_next <-- update_path_to_treekem cs (l-1) (if dir = Left then pow2 (l-1) else n - (pow2 (l-1))) next_i group_context next_update_path;
+      path_data <-- update_path_node_to_treekem cs group_context dir head_update_path_nodes;
+      return (PNode path_data path_next)
+    )
   )
 
 (*** ratchet_tree extension (11.3) ***)
